Correctness of "with" statements proven.

LambdaS5/coq/EjsToLjs.v
@@ -20,7 +20,7 @@ End EjsToLjsHelper.
 
 Definition make_builtin s := L.expr_id s.
 
-Definition context := make_builtin "%context".
+Definition context := make_builtin "$context".
 
 Definition eq e1 e2 := L.expr_op2 L.binary_op_stx_eq e1 e2.
 
@@ -61,10 +61,10 @@ Definition make_set_field obj fld v :=
     with_error_dispatch (make_app_builtin "%set-property" [to_object obj; to_string fld; v]).
 
 Definition make_var_set fld v :=
-    make_app_builtin "%EnvCheckAssign" [L.expr_id "%context"; L.expr_string fld; v; L.expr_id "%strict"].
+    make_app_builtin "%EnvCheckAssign" [L.expr_id "$context"; L.expr_string fld; v; L.expr_id "$strict"].
 
 Definition make_var_id i :=    
-    make_app_builtin "%EnvGet" [L.expr_id "%context"; L.expr_string i; L.expr_id "%strict"].
+    make_app_builtin "%EnvGet" [L.expr_id "$context"; L.expr_string i; L.expr_id "$strict"].
 
 Definition make_getter e := make_app_builtin "%MakeGetter" [e].
 
@@ -116,22 +116,22 @@ Definition make_throw e :=
     L.expr_throw (make_app_builtin "%JSError" [e]).
 
 Definition make_with e1 e2 := 
-    L.expr_let "%context" (make_app_builtin "%newObjEnvRec" [context; e1; L.expr_true]) e2.
+    L.expr_let "$context" (make_app_builtin "%newObjEnvRec" [context; to_object e1; L.expr_true]) e2.
 
-Definition if_strict e1 e2 := L.expr_if (L.expr_id "%strict") e1 e2.
+Definition if_strict e1 e2 := L.expr_if (L.expr_id "$strict") e1 e2.
 
 Definition syntax_error s := make_app_builtin "%SyntaxError" [L.expr_string s].
 
 Definition store_parent_in e :=
-    L.expr_let "%parent" context e.
+    L.expr_let "$parent" context e.
 
 Definition new_context_in ctx e :=
-    L.expr_let "%context" ctx e.
+    L.expr_let "$context" ctx e.
 
 Definition derived_context_in flds e :=
     let objattrs := L.objattrs_intro (L.expr_string "DeclEnvRec") 
-        L.expr_true L.expr_null L.expr_undefined (L.expr_id "%parent") in
-    new_context_in (L.expr_object objattrs nil flds) e.
+        L.expr_true L.expr_null L.expr_undefined L.expr_null in
+    new_context_in (L.expr_object objattrs [("parent", L.expr_id "$parent")] flds) e.
 
 Definition make_var_decl is e := 
     let flds := List.map (fun ip => 
@@ -139,10 +139,10 @@ Definition make_var_decl is e :=
     derived_context_in flds e.
 
 Definition make_strictness b e := 
-    L.expr_let "%strict" (L.expr_bool b) e.
+    L.expr_let "$strict" (L.expr_bool b) e.
 
 Definition make_resolve_this e :=
-    make_app_builtin "%resolveThis" [L.expr_id "%strict"; e].
+    make_app_builtin "%resolveThis" [L.expr_id "$strict"; e].
 
 Definition make_lambda f (is : list string) p := 
     let 'E.prog_intro str vis e := p in 
@@ -151,9 +151,9 @@ Definition make_lambda f (is : list string) p :=
         map (fun p => let '(vnum, vid) := p in (vid, L.expr_get_field (L.expr_id "%args") (L.expr_string vnum))) 
             (zipl_stream (id_stream_from 0) is) in
     let vdecls := map (fun i => (i, L.expr_undefined)) vis in
-    L.expr_lambda ["%this"; "%args"] (
+    L.expr_lambda ["$this"; "%args"] (
     L.expr_label "%ret" (
-    L.expr_let "%this" (make_resolve_this (L.expr_id "%this")) (
+    L.expr_let "$this" (make_resolve_this (L.expr_id "$this")) (
     make_var_decl (vdecls ++ ("arguments", make_app_builtin "%mkArgsObj" [args_obj]) :: argdecls) (
     make_strictness str (
     L.expr_seq (f e) L.expr_undefined))))).
@@ -162,7 +162,7 @@ Definition make_fobj f is p (ctx : L.expr) :=
     ifb Exists (fun nm => nm = "arguments" \/ nm = "eval") is \/ Has_dupes is then 
         if_strict (syntax_error "Illegal function definition") L.expr_undefined else
     store_parent_in (make_app_builtin "%MakeFunctionObject" 
-        [make_lambda f is p; L.expr_number (length is); L.expr_id "%strict"]).
+        [make_lambda f is p; L.expr_number (length is); L.expr_id "$strict"]).
 
 Definition make_rec_fobj f i is p ctx :=
     let fobj := make_fobj f is p ctx in
@@ -266,7 +266,7 @@ Definition make_app f (e : E.expr) es :=
     let args_obj := make_args_obj es in 
     match e with
     | E.expr_var_id "eval" =>
-        make_app_builtin "%maybeDirectEval" [L.expr_id "%this"; L.expr_id "%context"; args_obj; L.expr_id "%strict"]
+        make_app_builtin "%maybeDirectEval" [L.expr_id "$this"; L.expr_id "$context"; args_obj; L.expr_id "$strict"]
     | E.expr_get_field obj fld =>
         make_app_builtin "%AppMethod" [f obj; f fld; args_obj]
     | _ => 
@@ -356,7 +356,7 @@ Fixpoint ejs_to_ljs (e : E.expr) : L.expr :=
     | E.expr_var_id i => make_var_id i
 (*    | E.expr_var_decl is e => make_var_decl is (ejs_to_ljs e) *)
     | E.expr_var_set i e => make_var_set i (ejs_to_ljs e)
-    | E.expr_this => make_builtin "%this"
+    | E.expr_this => make_builtin "$this"
     | E.expr_object ps => make_object (List.map (fun (p : string * E.property) => let (a,b) := p in (a, property_to_ljs b)) ps) 
     | E.expr_array es => make_array (List.map ejs_to_ljs es)
     | E.expr_app e es => make_app ejs_to_ljs e (List.map ejs_to_ljs es)
@@ -404,5 +404,5 @@ Definition init_global i :=
 
 Definition ejs_prog_to_ljs ep :=
     let 'E.prog_intro strict is inner := ep in
-    L.expr_let "%context" (L.expr_id (if strict then "%strictContext" else "%nonstrictContext")) 
+    L.expr_let "$context" (L.expr_id (if strict then "%strictContext" else "%nonstrictContext")) 
         (L.expr_seq (L.expr_seqs (List.map init_global is)) (make_strictness strict (ejs_to_ljs inner))). 
